# 10.2

## 题

设 $N^4_i(x)\ (i=1,2)$ 为四阶规范 $B$ 样条，节点序列 $\{y_i\}_{i=1}^6$ 为 $\{1,2,3,5,6,8\}$，令 $s(x)=4N^4_1(x)+6N^4_2(x)$ 

(1) 求 $s(x)$ 在区间 $[2,3]$ 上的 Bezier 表示

(2) 计算 $s(2)$，$s(2.5)$，$s^\prime(3)$ 的值

## 解

节点序列扩充为 $\{y_i\}_{i=-1}^7$，满足 $y_{-1}<y_0<y_1<\dots<y_6<y_7$，则 $s(x)=\sum_{i=-1}^3c_iN^4_i(x)$，其中 $c_{-1}=0,c_0=0,c_1=4,c_2=6,c_3=0$  

### (1)

设 $p(x)=s(x)|_{[2,3]}$，$f(x_1,x_2,x_3)$ 是 $p(x)$ 的开花，且
$$
p(x)=\sum_{i=0}^3b_iB^3_i(x-2)
$$
其中
$$
\begin{aligned}
B^3_i(x-2)&=\mathrm{C}_3^i(x-2)^i(3-x)^{3-i}\\
b_0&=f(2,2,2)\\
b_1&=f(2,2,3)\\
b_2&=f(2,3,3)\\
b_3&=f(3,3,3)
\end{aligned}
$$
由定理 10.4 可知
$$
\begin{aligned}
f(y_0,1,2)&=c_{-1}=0\\
f(1,2,3)&=c_0=0\\
f(2,3,5)&=c_1=4\\
f(3,5,6)&=c_2=6
\end{aligned}
$$

根据极形式的性质知
$$
\begin{aligned}
f(1,2,2)&=\frac{1}{3-y_0}f(y_0,1,2)+\frac{2-y_0}{3-y_0}f(1,2,3)=0\\
b_1=f(2,2,3)&=\frac{3}{4}f(1,2,3)+\frac{1}{4}f(2,3,5)=1\\
b_2=f(2,3,3)&=\frac{1}{2}f(1,2,3)+\frac{1}{2}f(2,3,5)=2\\
f(3,3,5)&=\frac{3}{4}f(2,3,5)+\frac{1}{4}f(3,5,6)=\frac{9}{2}\\
b_0=f(2,2,2)&=\frac{1}{2}f(1,2,2)+\frac{1}{2}f(2,2,3)=\frac{1}{2}\\
b_3=f(3,3,3)&=\frac{2}{3}f(2,3,3)+\frac{1}{3}f(3,3,5)=\frac{17}{6}\\
\end{aligned}
$$

> **测试** 
>
> ```matlab
> close all;
> x=2:0.001:3;
> t=[1,2,3,5,6,8];
> s=@(x) 4*N(t(1:5),x)+6*N(t(2:6),x);
> b=[0.5,1,2,17/6];
> p=@(x) sum(Elem(@(i) b(i+1)*Bernstein(3,i,x-2),0:3));
> plot(x,Elem(s,x),'r','linewidth',4);
> hold on;
> plot(x,Elem(p,x),'b','linewidth',2);
> ```

### (2)

记 $c_{i}^{[0]}=c_i\quad (i=-1,0,1,2,3)$ 

![image-20191215030748167](assets/image-20191215030748167.png)

则

$s(2)=c^{[3]}_2(2)=\frac{1}{2}$，$s(2.5)=c^{[3]}_2(2.5)=\frac{37}{24}$ 

---

![image-20191215034211049](assets/image-20191215034211049.png)

其中
$$
\begin{aligned}
c_1^{[1]}&=\frac{(m-1)\left(c_1^{[0]}-c_0^{[0]}\right)}{y_4-y_1}=3\\
c_2^{[1]}&=\frac{(m-1)\left(c_2^{[0]}-c_1^{[0]}\right)}{y_5-y_2}=\frac{3}{2}\\
c_3^{[1]}&=\frac{(m-1)\left(c_3^{[0]}-c_2^{[0]}\right)}{y_6-y_3}=-\frac{18}{5}\\
\end{aligned}
$$
$s^\prime(3)=c^{[3]}_3(3)=\frac{5}{2}$ 

# 10.3

## 题

设 $k\in\mathbb{Z}_+$，将 $(x-k)^{m-1}_+$ 展成 $\{N^m(x-i)\}_{i=-\infty}^{+\infty}$ 的级数，即求 $c_i$ 使得
$$
(x-k)^{m-1}_+=\sum_{i=-\infty}^{+\infty}c_iN^m(x-i)
$$

## 解

取 $y_i=i$，则 $N^m(x-i)=N^m_i(x)$，则 $(x-k)^{m-1}_+=\sum_{i=-\infty}^{+\infty}c_iN^m(x-i)=\sum_{i=-\infty}^{+\infty}c_iN^m_i(x)$ 

取 $k=0$，设 $t^{m-1}_+=\sum_{i=0}^{\infty}d_iN^m_i(t)$，当 $t>0$ 时，极形式为 $f(t_1,\dots,t_{m-1})=t_1\dots t_{m-1}$，则
$$
d_i=f(y_{i+1},\dots,y_{i+m-1})=\prod_{j=1}^{m-1}(i+j) \quad(i=0,1,\dots)
$$
由于 $N^m_i(t)$ 支集为 $[i,i+m]$，故 $d_i=0\ (i<0)$ 

则
$$
t^{m-1}_+=\sum_{i=0}^{\infty}d_iN^m_i(t)
$$
令 $t=x-k$，得
$$
(x-k)^{m-1}_+=\sum_{i=0}^{\infty}d_iN^m_i(x-k)=\sum_{i=0}^{\infty}d_iN^m_{i+k}(x)=\sum_{i=k}^{+\infty}c_iN^m_i(x)=\sum_{i=k}^{+\infty}c_iN^m_i(x-i)
$$
其中
$$
c_i=d_{i-k}=\prod_{j=1}^{m-1}(i-k+j)\quad(i=k,k+1,\dots)
$$
另 $c_i=0\ (i<k)$ 

